\documentclass[a4paper,9pt,twocolumn]{extarticle}

\usepackage[hmargin=0.75in,vmargin=0.75in]{geometry}
\setlength{\parskip}{1ex plus 0.5ex minus 0.5ex}
\usepackage{relsize}
\usepackage{exscale}
\usepackage[english]{babel}
\usepackage{parskip}
\usepackage{color}
\usepackage{algorithm,algorithmic}
\usepackage{amsmath,amsthm,amssymb,amsfonts}

\newcommand{\Diff}{\mathcal{D}}
\newcommand{\TODO}[1]{\textcolor{red}{#1}}

\makeatletter
\thm@headfont{\sc}
\newtheorem{theorem}{Theorem}

\title{Implicit Integrator}
\author{Jiong Chen}

\begin{document}
\maketitle

Euler-Lagrange equation:
\begin{equation}
	M\ddot u + D(u)\dot u - f_{int}(u) = f_{ext} \label{euler}
\end{equation}
with position constraint:
\begin{equation}
 Cu = u_c \label{cons}
\end{equation}
Rewrite equation \eqref{euler} as two ODEs together with \eqref{cons} and use Lagrangian multipliers, we have
\begin{equation*}
  \left\{
   \begin{aligned}
			v &= \dot u \\
			M\dot v + D(u)v - f_{int}(u) + C^T\lambda &= f_{ext} \\
			Cu &= u_c 
   \end{aligned}
   \right.
  \end{equation*}
Discretize above equations:
\begin{equation*}
  \left\{
   \begin{aligned}
			u_{k+ 1} &= u_k + hv_{k+1} \\
			M\frac{v_{k+1} - v_k}{h} + D(u_{k+1})v_{k+1}  + C^T\lambda &= f_{ext} + f_{int}(u_{k+1})\\
			Cu_{k+1} &= u_c 
   \end{aligned}
   \right.
  \end{equation*}
\begin{equation*}
M\frac{v_{k+1} - v_k}{h} + D(\TODO{u_k})v_{k+1}  + C^T\lambda = f_{ext} + f_{int}(u_k + hv_{k + 1})
\end{equation*}
\begin{equation*}
M\frac{v_{k+1} - v_k}{h} + \left[\alpha M + \beta K(u_k)\right]v_{k+1}  + C^T\lambda = f_{ext} + f_{int}(u_k + hv_{k + 1})
\end{equation*}
\begin{equation*}
M\frac{v_{k+1} - v_k}{h} + \left[\alpha M + \beta K(u_k)\right]v_{k+1}  + C^T\lambda \approx f_{ext} \TODO{- \frac{\partial E}{\partial x}\bigg|_{u_k} - K(u_k) hv_{k +1}}
\end{equation*}
\begin{eqnarray*}
\big((1 + h\alpha )M + (h\beta + h^2)K(u_k) \big )v_{k + 1} + C^T \lambda &=& Mv_k + h(f_{ext} - \frac{\partial E}{\partial x}\bigg|_{u_k}) \\
Cv_{k + 1} &=& \frac{1}{h} (u_c - Cu_k)
\end{eqnarray*}
\begin{equation*}
\begin{bmatrix}
	(1 + h\alpha )M + (h\beta + h^2)K(u_k)  & C^T \\
	C & 0
\end{bmatrix}
\begin{bmatrix}
	v_{k + 1} \\
	\lambda
\end{bmatrix}
=
\begin{bmatrix}
	Mv_k + h(f_{ext} - \frac{\partial E}{\partial x}\bigg|_{u_k})  \\
	\frac{1}{h} (u_c - Cu_k)
\end{bmatrix}
\end{equation*}

 
\end{document}
